
---
title: Coupled enhancer-promoter condensates
date-format: YYYY-MM-DDTHH:mm:ssZ
preview:
    port: 4200
    browser: false
---
## Dimensional Asymmetric Double-Well
$$F_{DW}(\rho_p , a , b)+\cdots = \int d^2x \bigg[\rho_p (\phi_p -a)^2(\phi_p -b)^2-\chi \phi_p \phi_r+c \phi_p^2 \phi_r^2+\rho_r\phi_r^2+\frac{\kappa}{2}(\nabla\phi_p)^2\bigg]$$

With $a<b$, $a =0.1$, $b = 0.7$, $\phi_{p,+}=0.63$, $\phi_{p,-}=0.13$, and $\rho_p = 1$.

## Dimensional Symmetric Double-Well
$$\begin{aligned}
F_{DW}(c_0 , \alpha, \beta)+\cdots &= \int d^2x \bigg[\frac{\alpha}{4}(c-c_0)^4+\frac{\beta}{2}(c-c_0)^2+\frac{\lambda}{2}m^2 +\gamma m c\\
&+\frac{\kappa}{2}(\nabla c)^2- \chi_{PD} \exp (- |\vec r - \vec r_e |^2/2 \sigma^2) c \bigg]+ \frac{3k_B T}{2L_CL_P}|\vec r_e - \vec r_p|^2
\end{aligned}$$


##  Symmetric PFStability Non-Dimensional
$$\tilde F_{DW}(\bar c_1, \tilde \beta) +\cdots= \int d^2x \bigg[\frac{1}{4}(\tilde c_1-\bar c_1)^4+\frac{\tilde \beta}{2}(\tilde c_1-\bar c_1)^2+\frac{\tilde \lambda}{2}c_2^2 +\tilde \gamma c_1 c_2+\frac{\tilde \kappa}{2}|\nabla c_1|^2-\tilde \chi_{PD} \exp (- |\vec r - \vec r_0 |^2/2 \sigma^2)\tilde c_1\bigg]+ \frac{\tilde k}{2}|\vec r_e - \vec r_p|$$

## Symmetric Binodal Points

$$\begin{aligned}
\frac{\partial}{\partial c}\left[\frac{\alpha}{4}(c-c_0)^4+\frac{\beta}{2}(c-c_0)^2\right]&=0\\
\alpha(c-c_0)^3+\beta (c-c_0)&=0\\
\alpha (c-c_0)\left(c-c_0+\sqrt{-\beta/\alpha}\right)\left(c-c_0-\sqrt{-\beta/\alpha}\right)&=0
\end{aligned}$$
$$c = c_0 \pm \sqrt{-\beta/\alpha}$$

## Asymmetric-Symmetric Conversion (Dimensional)

$$\begin{aligned}
\rho_p (\phi_p -a)^2(\phi_p -b)^2&= \rho_p (\phi_p^2 - 2a \phi_p+a^2)(\phi_p^2 - 2b \phi_p+b^2)\\
&=\rho_p (\phi_p^4 +(-2a -2 b)\phi_p ^3+(a^2 + b^2 +4ab)\phi_p^2 \\
&+(-2a^2 b -2a b^2)\phi_p+a^2b^2)\\
&=\rho_p\phi_p^4 +\rho_p(-2a -2 b)\phi_p ^3+\rho_p(a^2 + b^2 +4ab)\phi_p^2 \\
&+\rho_p(-2a^2 b -2a b^2)\phi_p+\rho_pa^2b^2\\
\end{aligned}$$

$$\begin{aligned}
\frac{\alpha}{4}(c-c_0)^4+\frac{\beta}{2}(c-c_0)^2& = \frac{\alpha}{4}(c^4-4c_0c^3+6c_0^2c^2-4c_0^3c+c_0^4)+ \frac{\beta}{2}(c^2 - 2c_0c+c_0^2)\\
& = \left(\frac{\alpha}{4}\right)c^4 +\left(-\alpha c_0 \right)c^3 + \left(\frac{3}{2}\alpha c_0^2+\frac{\beta}{2}\right)c^2\\
&+\left(-\alpha c_0^3 -\beta c_0 \right)c + \left(\frac{\alpha}{4}c_0^4+\frac{\beta}{2}c_0^2\right)
\end{aligned}$$

$$\rho_p= \frac{\alpha}{4}$${#eq-match1}
$$\rho_p (-2a -2b)= -\alpha c_0$${#eq-match2}
$$\rho_p(a^2 + b^2 +4ab)=\frac{3}{2}\alpha c_0^2+\frac{\beta}{2}$${#eq-match3}
$$\rho_p(-2a^2 b -2a b^2) = \left(-\alpha c_0^3 -\beta c_0 \right)$${#eq-match4}
<!-- $$-\rho_p 2ab(a+b)=-c_0 (\alpha c_0^2+\beta)$$ -->
$$\rho_pa^2b^2=\left(\frac{\alpha}{4}c_0^4+\frac{\beta}{2}c_0^2\right)$${#eq-match5}

Substitute @eq-match1 to @eq-match2.
$$\frac{\alpha}{4}(-2a-2b)=-\alpha c_0$$
$$c_0 = \frac{a+b}{2}$${#eq-c0}
Substitute @eq-c0 to @eq-match4.
$$\rho_p 2ab(a+b)=\frac{a+b}{2} \left[\alpha \left(\frac{a+b}{2}\right)^2 + \beta\right]$$

$$16\rho_p ab=\alpha (a^2+2ab+b^2) + 4\beta$$ {#eq-from64}
Substitute @eq-from64 to @eq-match3
$$\rho_p(a^2 + b^2 +4ab)=\frac{3}{2}\alpha \left(\frac{a+b}{2}\right)^2+\frac{\beta}{2}$$

$$8\rho_p(a^2 + b^2 +4ab)=3\alpha \left(a^2+2ab+b^2\right)+4\beta$$ {#eq-from643}

Subtract @eq-from64 and @eq-from643.

$$8 \rho_pa^2 + 8 \rho_p b^2 +16 \rho_p ab=2\alpha (a^2 + 2ab + b^2)$$

$$\alpha =\frac{8 \rho_pa^2 + 8 \rho_p b^2 +16 \rho_p ab}{2(a^2 + 2ab + b^2)}=\frac{8\rho_p (a+b)^2}{2(a+b)^2}= 4\rho_p $$

This is consistent with @eq-match1. Substitute to @eq-from64.

$$16\rho_p ab=4 \rho_p (a^2+2ab+b^2) + 4\beta$$

$$-4 \rho_p (a^2-2ab+b^2)= 4\beta$$

$$\beta=-\rho_p (a-b)^2$$ {#eq-beta}
We have used [@eq-match1;@eq-match2;@eq-match4]. Check with [@eq-match3;@eq-match5].

For @eq-match3:
$$LHS=\rho_p(a^2 + b^2 +4ab)$$

$$\begin{aligned}
RHS&=\frac{3}{2}\alpha c_0^2+\frac{\beta}{2} = \frac{3}{2}(4 \rho_p )\left(\frac{a+b}{2}\right)^2-\frac{\rho_p (a-b)^2}{2}\\
&=\frac{3}{2}\rho_p (a+b)^2-\frac{\rho_p}{2} (a-b)^2=\rho_p (a^2+4ab+b^2)
\end{aligned}$$

$LHS=RHS$ consistent with @eq-match3.

For @eq-match5:
$$LHS=\rho_pa^2b^2$$

$$\begin{aligned}
RHS&=\left(\frac{\alpha}{4}c_0^4+\frac{\beta}{2}c_0^2\right)= \rho_p \frac{(a+b)^4}{16}-\frac{\rho_p}{2}(a-b)^2\frac{(a+b)^2}{4}\\
& = \frac{\rho_p}{16} (a+b)^2\left[(a+b)^2-2(a-b)^2\right]
\end{aligned}$$

$$LHS \neq RHS$$

Equations differ by a scalar, which is not important in free energy gradients.

$$LHS-RHS = \rho_p \left[a^2b^2 - \frac{1}{16} (a+b)^2\left\{(a+b)^2-2(a-b)^2\right\}\right]$$

Hence,
$$\begin{cases}
\alpha = 4 \rho_p\\
\beta = -\rho_p (a-b)^2\\
c_0 = 0.5(a+b)
\end{cases}$$


Likewise,
$$\begin{cases}
\rho_p = 0.25 \alpha\\
a =c_0 - \sqrt{-\beta/\alpha}\\
b = c_0 + \sqrt{-\beta/\alpha}
\end{cases}$$

## Non-dimensionalize Symmetric Double-Well
Use the following characteristic scales
$$\begin{aligned}\
[C]&=(c_0/\bar c)&
[T]&=\frac{1}{k_d}&
[L]&=\sqrt{M_m\lambda/k_d}&
[E]&=[\alpha][C]^4[L^2]&
\end{aligned}$$


This is a functional derivative

$$\partial_t c=M_c\nabla^2\left(\frac{\delta F}{\delta c}\right)=M_c\nabla^2\left(\alpha (c-c_0)^3 + \beta (c-c_0)+ \gamma m -k \nabla^2 c\right)$$
$$\partial_t m=M_m\lambda\nabla^2 m+k_p(\vec{r})c-k_dm$$

$$\begin{aligned}\tilde c &= \frac{c}{c_0/\bar c}&
\tilde m &= \frac{m}{c_0/\bar c}&
\tilde t  &= k_d t&
k  &= \frac{k_p}{k_d}&
\tilde{r} &= \frac{r}{l_{\text{RNA}}}=\frac{r}{\sqrt{M_m \lambda/k_d}}
\end{aligned}$$


$$\partial_{\tilde t} \tilde c=\frac{M_c}{k_d}\nabla^2\left(\alpha (c_0/\bar c)^2(\tilde c-\bar c)^3 + \beta (\tilde c-\bar c)+ \gamma \tilde m -\kappa \nabla^2 \tilde c\right)$$

$$\partial_{\tilde t} \tilde c=\frac{M_c\alpha (c_0/\bar c)^2}{M_m \lambda}\tilde \nabla^2\left((\tilde c-\bar c)^3 + \beta\frac{1}{\alpha (c_0/\bar c)^2} (\tilde c-\bar c)+ \gamma\frac{1}{\alpha (c_0/\bar c)^2} \tilde m -\kappa \frac{1}{\alpha (c_0/\bar c)^2 } \frac{k_d}{M_m}\tilde \nabla^2 \tilde c\right)$$

$$\partial_{\tilde t} \tilde c=M\tilde \nabla^2\left((\tilde c-\bar c)^3 +\tilde \beta (\tilde c-\bar c)+ \tilde \gamma \tilde m - \tilde \kappa \nabla^2 \tilde c\right)$$

$$\begin{aligned}
M &= \frac{M_c\alpha (c_0/\bar c)^2}{M_m \lambda}&
\tilde \beta &= \beta\frac{1}{\alpha (c_0/\bar c)^2}&
\tilde \gamma &= \gamma\frac{1}{\alpha (c_0/\bar c)^2}&
\tilde \kappa &= \frac{\kappa }{\alpha (c_0/\bar c)^2}\frac{k_d}{M_m}
\end{aligned}$$

$$\partial_{\tilde t} \tilde m=\frac{M_m\lambda}{k_d}\tilde \nabla^2 \tilde m+k\tilde c-\tilde m$$

$$\partial_{\tilde t} \tilde m=\tilde \nabla^2 \tilde m+k\tilde c-\tilde m$$


<!-- $$\begin{aligned}
F&=\frac{\alpha}{4}(c-c_0)^4+\frac{\beta}{2}(c-c_0)^2\\
\frac{F}{\alpha}&= \frac{1}{4}(c-c_0)^4+\frac{1}{2}\frac{\beta}{\alpha}(c-c_0)^2\\
F&=C^4\left[\frac{1}{4}\left(\frac{c}{C}-\frac{c_0}{C}\right)^4+\frac{1}{2}\frac{1}{C^2}\frac{\beta}{\alpha}\left(\frac{c}{C}-\frac{c_0}{C}\right)^2\right]\\
\frac{F}{C^4}&=\left[\frac{1}{4}\left(\frac{c}{C}-\frac{c_0}{C}\right)^4+\frac{1}{2}\frac{\beta}{C^2\alpha}\left(\frac{c}{C}-\frac{c_0}{C}\right)^2\right]
\end{aligned}$$


Hence, 
$$\tilde c_1 = \frac{a+b}{2C}$$
$$\tilde \beta =\frac{-(a-b)^2}{4C^2}$$ -->



## Dimensionless Enhancer Dynamics

Notice the change in notation from the dimensional to dimensionless equation. I'm shifting the notation form Pradeep's notes to the documentation in the PFStability code.

$$\begin{aligned}
F_{DW}(c_0 , \alpha, \beta) &= \int d^2x \bigg[\frac{\alpha}{4}(c-c_0)^4+\frac{\beta}{2}(c-c_0)^2+\frac{\lambda}{2}m^2 +\gamma m c\\
&+\frac{\kappa}{2}(\nabla c)^2- \chi_{PD} \exp (- |\vec r - \vec r_e |^2/2 \sigma^2) c \bigg]+ \frac{3k_B T}{2L_CL_P}|\vec r_e - \vec r_p|^2
\end{aligned}$$

$$\begin{aligned}
\tilde F(\tilde c_1,\tilde c_2,\vec r_e)&=\frac{F}{\alpha (c_0/\bar c)^4 (M_m\lambda/k_d)}= \int d^2{\tilde x} \bigg[\frac{1}{4}(\tilde c_1-\bar c_1)^4+\frac{\tilde \beta}{2}(\tilde c_1-\bar c_1)^2+\frac{\tilde \lambda}{2}\tilde c_2^2 +\tilde \gamma \tilde c_1 \tilde c_2+\frac{\tilde \kappa}{2}|\tilde \nabla \tilde c_1|^2\\
&-\tilde \chi_{PD} \exp (- |\vec {\tilde r} - \vec {\tilde r_e} |^2/2 \tilde \sigma^2)\tilde c_1 \bigg]+ \frac{\tilde k}{2}|\vec {\tilde r_e} - \vec {\tilde r_p}|^2
\end{aligned}$$

Recall our characteristic concentration, time, length, and energy scales. Note that $\bar c$ is dimensionless.
$$\begin{aligned}\ [\bar c]&=1&
[C]&=(c_0/\bar c)&
[T]&=\frac{1}{k_d}&
[L]&=\sqrt{M_m\lambda/k_d}&
[E]&=[\alpha][C]^4[L^2] \end{aligned}$$

$$F =  [E]\tilde F = \alpha (c_0/\bar c)^4 (M_m\lambda/k_d) \tilde F$$

$$[\chi_{PD}]=\frac{[E]}{[L]^2[C]}=[\alpha][C^3]=\alpha(c_0/\bar c)^3$$

$$\chi_{PD}=[\chi_{PD}]\tilde c=\alpha(c_0/\bar c)^3\tilde c$$


$$[M_D]=\frac{[\partial_{\vec r_e}]}{[\nabla _{\vec x_e}F]}=\frac{[L]/[T]}{[E]/[L]}=\frac{[L]^2}{[E][T]}=\frac{[L]^2}{[\alpha][C]^4[L^2][T]}=\frac{1}{[\alpha][C]^4[T]}= \frac{k_d}{\alpha (c_0/\bar c)^4}$$

$$M_D = [M_D] \tilde M_D = \frac{k_d}{\alpha (c_0/\bar c)^4} \tilde M_D$$

This is a partial derivative (gradient)
$$\partial_t\vec r_e=-M_D\vec \nabla_{\vec r_e}F=M_D \int d^2 x \left[\chi_{PD}c_1\left(\frac{\vec r - \vec r_e}{\sigma^2}\right)\exp \left(- \frac{|\vec r - \vec r_e|^2}{2 \sigma^2}\right)\right]- M_D \frac{3 k_B T}{L_P L_C} (\vec r_e - \vec r_p)$$

$$\begin{aligned}
k_d\left(\sqrt{M_m\lambda/k_d}\right)\partial_{\tilde t}{\vec {\tilde r_e}} &= M_D \int d^2 {\tilde x} (M_m\lambda/k_d) \bigg[\chi_{PD}c_1\bigg(\frac{1}{\sqrt{M_m\lambda/k_d}}\frac{\vec {\tilde r} - \vec {\tilde r_e}}{{\tilde \sigma}^2}\bigg)\exp \bigg(- \frac{|\vec {\tilde r}-\vec {\tilde r_e}|^2}{2 {\tilde \sigma}^2}\bigg)\bigg]\\
&- M_D  \frac{3 k_B T}{L_P  L_C}  \left( \sqrt{M_m\lambda/k_d}\right) (\vec {\tilde r_e} - \vec {\tilde r_p})
\end{aligned}$$


$$\partial_{\tilde t}{\vec {\tilde r_e}} = \frac{M_D}{k_d} \int d^2 {\tilde x} \left[\chi_{PD}c_1\left(\frac{\vec {\tilde r} - \vec {\tilde r_e}}{{\tilde \sigma}^2}\right)\exp \left(- \frac{|\vec {\tilde r} - \vec {\tilde r_e}|^2}{2 {\tilde \sigma}^2}\right)\right]- \frac{M_D}{k_d} \frac{3 k_B T}{ L_PL_C}  (\vec {\tilde r_e} - \vec {\tilde r_p})$$

$$\begin{aligned}
\partial_{\tilde t}{\vec {\tilde r_e}} &= \left\{\frac{M_D \alpha (c_0/\bar c)^4}{k_d}\right\} \int d^2 {\tilde x} \left[ \left\{\frac{\chi_{PD}}{\alpha (c_0/\bar c)^3}\right\} \left\{\frac{c_1}{(c_0/\bar c)}\right\}\left(\frac{\vec {\tilde r} - \vec {\tilde r_e}}{{\tilde \sigma}^2}\right)\exp \left(- \frac{|\vec {\tilde r} - \vec {\tilde r_e}|^2}{2 {\tilde \sigma}^2}\right)\right]\\
&-  \left\{\frac{M_D  \alpha (c_0/\bar c)^4}{k_d}\right\}  \left\{\frac{3 k_B T}{ L_PL_C }\frac{1}{\alpha (c_0/\bar c)^4}\right\}  (\vec {\tilde r_e} - \vec {\tilde r_p})
\end{aligned}$$


$$\partial_{\tilde t}{\vec {\tilde r_e}} =  \tilde M_D \int d^2 {\tilde x} \left[\tilde \chi_{PD}\tilde c_1\left(\frac{\vec {\tilde r} - \vec {\tilde r_e}}{{\tilde \sigma}^2}\right)\exp \left(- \frac{|\vec {\tilde r} - \vec {\tilde r_e}|^2}{2 {\tilde \sigma}^2}\right)\right]- \tilde M_D  \tilde k  (\vec {\tilde r_e} - \vec {\tilde r_p})$$

$$\begin{aligned}
\tilde M_D &= \frac{M_D \alpha (c_0/\bar c)^4}{k_d}&
\tilde k &= \frac{3 k_B T}{L_PL_C }\frac{1}{\alpha (c_0/\bar c)^4}&
\tilde c &= \frac{\chi_{PD}}{\alpha (c_0/\bar c)^3}&
\end{aligned}$$


## Protein/RNA Coupled Dynamics
$$\tilde F= \int d^2x \bigg[\frac{1}{4}(\tilde c_1-\bar c_1)^4+\frac{\tilde \beta}{2}(\tilde c_1-\bar c_1)^2+\frac{\tilde \lambda}{2}{\tilde c_2}^2 +\tilde \gamma \tilde c_1 \tilde c_2+\frac{\tilde \kappa}{2}|\tilde \nabla \tilde c_1|^2-\tilde \chi_{PD} \exp (- |\vec {\tilde r} - \vec {\tilde r_0} |^2/2 {\tilde \sigma}^2)\tilde c_1\bigg]+ \frac{\tilde k}{2}|\vec {\tilde r_e} - \vec {\tilde r_p}- \vec {\tilde l}|$$

$$\partial_{\tilde t} \tilde c_1=M\tilde \nabla^2\left((\tilde c_1-\bar c)^3 +\tilde \beta (\tilde c_1-\bar c)+ \tilde \gamma \tilde c_2 - \tilde \kappa \nabla^2 \tilde c_1-\tilde \chi_{PD}\exp (- |\vec {\tilde r} - \vec {\tilde r_0} |^2/2 {\tilde \sigma}^2)\right)$$
$$\partial_{\tilde t} \tilde c_2=\tilde \nabla^2 \tilde c_2+k\tilde c_1-\tilde c_2$$
$$\partial_{\tilde t}{\vec {\tilde r_e}} =  \tilde M_D \int d^2 {\tilde x} \left[\tilde \chi_{PD}\tilde c_1\left(\frac{\vec {\tilde r} - \vec {\tilde r_e}}{{\tilde \sigma}^2}\right)\exp \left(- \frac{|\vec {\tilde r} - \vec {\tilde r_e}|^2}{2 {\tilde \sigma}^2}\right)\right]- \tilde M_D  \tilde k  (\vec {\tilde r_e} - \vec {\tilde r_p}- \vec {\tilde l})$$

## Protein-Enhancer Coupling Steady State

$$0 =  \tilde M_D \int d^2 {\tilde x} \left[\tilde \chi_{PD}\tilde c_1\left(\frac{\vec {\tilde r} - \vec {\tilde r_e}}{{\tilde \sigma}^2}\right)\exp \left(- \frac{|\vec {\tilde r} - \vec {\tilde r_e}|^2}{2 {\tilde \sigma}^2}\right)\right]- \tilde M_D  \tilde k  (\vec {\tilde r_e} - \vec {\tilde r_p}- \vec {\tilde l})$$
$$\frac{\tilde k}{\tilde \chi_{PD}} = \frac{ \displaystyle \int d^2 {\tilde x} \left[\tilde c_1\left(\frac{\vec {\tilde r} - \vec {\tilde r_e}}{{\tilde \sigma}^2}\right)\exp \left(- \frac{|\vec {\tilde r} - \vec {\tilde r_e}|^2}{2 {\tilde \sigma}^2}\right)\right]}{(\vec {\tilde r_e} - \vec {\tilde r_p}- \vec {\tilde l})}$$

![](_assets/SharpInterfaceEnhancer.png){width=300}


## Re-entrant term
$$\tilde F= \int d^2x \bigg[\frac{1}{4}(\tilde c_1-\bar c_1)^4+\frac{\tilde \beta}{2}(\tilde c_1-\bar c_1)^2+\frac{\tilde \lambda}{2}c_2^2 +\tilde \gamma c_1 c_2+\frac{\tilde \chi_{PR}}{2} c_1^2c_2^2+\frac{\tilde \kappa}{2}|\tilde \nabla c_1|^2-\tilde \chi_{PD} \exp (- |\vec r - \vec r_0 |^2/2 \sigma^2)\tilde c_1\bigg]+ \frac{\tilde k}{2}|\vec r_e - \vec r_p|$$

$$\partial_{\tilde t} \tilde c_1=M\tilde \nabla^2\left((\tilde c_1-\bar c)^3 +\tilde \beta (\tilde c_1-\bar c)+ \tilde \gamma \tilde c_2 + \tilde \chi_{PR} c_1c_2^2 - \tilde \kappa \tilde \nabla^2 \tilde c_1 - \tilde \chi_{PD}\exp (- |\vec {\tilde r} - \vec {\tilde r_0} |^2/2 {\tilde \sigma}^2)\right)$$

$$\partial_{\tilde t} \tilde c_2=\tilde \nabla^2 \tilde c_2+k\tilde c_1-\tilde c_2$$

$$J = \begin{bmatrix}\partial_{c_1^2}F & \partial_{c_1c_2}F\\ \partial_{c_2c_1}F & \partial_{c_2^2}F\end{bmatrix}$$

$$J = \begin{bmatrix}3(\tilde c_1 - \bar c)^2+\beta+\tilde \chi_{PR}c_2^2 & \tilde \gamma + 2 \tilde \chi_{PR} c_1 c_2\\ \tilde \gamma + 2\tilde \chi_{PR} c_1 c_2 & \tilde \chi_{PR}c_1^2\end{bmatrix}$$